Block.v
@@ -1,0 +1,573 @@
+(* This file is part of the LLIR Semantics project. *)
+(* Licensing information is available in the LICENSE file. *)
+(* (C) 2020 Nandor Licker. All rights reserved. *)
+
+Require Import Coq.ZArith.ZArith.
+Require Import Coq.Lists.List.
+Require Import FunInd.
+Require Import Recdef.
+
+Require Import LLIR.Dom.
+Require Import LLIR.LLIR.
+Require Import LLIR.Values.
+Require Import LLIR.Maps.
+
+Import ListNotations.
+
+Section FUNCTION.
+  Variable f: func.
+
+  Definition entry: node := f.(fn_entry).
+
+  Inductive BasicBlockHeader: node -> Prop :=
+    | block_header:
+      forall (header: node)
+        (REACH: Reachable f header)
+        (TERM: forall (term: node), SuccOf f term header -> TermAt f term)
+        (INST: f.(fn_insts) ! header <> None),
+        BasicBlockHeader header
+    .
+
+  Inductive BasicBlock: node -> node -> Prop :=
+    | bb_header:
+      forall (header: node)
+        (HEADER: BasicBlockHeader header),
+          BasicBlock header header
+    | bb_elem:
+      forall (header: node) (prev: node) (elem: node)
+        (NOT_HEADER: header <> elem)
+        (NOT_ENTRY: entry <> elem)
+        (NOT_PREV: prev <> elem)
+        (BLOCK: BasicBlock header prev)
+        (PRED: SuccOf f prev elem)
+        (NOT_TERM: ~TermAt f prev)
+        (INST: f.(fn_insts) ! elem <> None)
+        (NO_PHI: f.(fn_phis) ! elem = None)
+        (UNIQ: forall (prev': node), SuccOf f prev' elem -> prev' = prev),
+          BasicBlock header elem
+    .
+
+  Theorem bb_reaches:
+    forall (header: node) (elem: node),
+      BasicBlock header elem -> Reachable f elem.
+  Proof.
+    intros header elem Hbb.
+    induction Hbb.
+    inversion HEADER.
+    apply REACH.
+    apply reach_succ with (a := prev); auto.
+  Qed.
+
+  Theorem bb_has_header:
+    forall (header: node) (elem: node),
+      BasicBlock header elem -> BasicBlockHeader header.
+  Proof.
+    intros header elem Hbb.
+    induction Hbb.
+    apply HEADER.
+    apply IHHbb.
+  Qed.
+
+  Theorem bb_is_header:
+    forall (header: node),
+      BasicBlock header header -> BasicBlockHeader header.
+  Proof.
+    intros header Hbb.
+    inversion Hbb; auto; contradiction.
+  Qed.
+
+  Theorem bb_header_dom_nodes:
+    forall (header: node) (elem: node),
+      BasicBlock header elem -> Dominates f header elem.
+  Proof.
+    intros header elem Hbb.
+    induction Hbb. apply dom_self.
+    apply dom_trans with (m := prev); auto.
+    apply dom_step.
+    repeat split.
+    + apply bb_reaches with (header := header). apply Hbb.
+    + apply PRED.
+    + apply NOT_ENTRY.
+    + intros n Hsucc. symmetry. apply UNIQ. apply Hsucc.
+  Qed.
+
+  Theorem bb_header_unique:
+    forall (elem: node) (header: node) (header': node),
+      BasicBlock header elem ->
+      BasicBlock header' elem ->
+      header = header'.
+  Proof.
+    intros elem header header'.
+    intros Hbb Hbb'.
+    induction Hbb'.
+    {
+      inversion Hbb; auto.
+      inversion HEADER.
+      apply TERM in PRED.
+      apply NOT_TERM in PRED.
+      inversion PRED.
+    }
+    {
+      apply IHHbb'.
+      inversion Hbb.
+      {
+        subst.
+        inversion HEADER.
+        apply TERM in PRED.
+        apply NOT_TERM in PRED.
+        inversion PRED.
+      }
+      {
+        subst.
+        apply UNIQ in PRED0.
+        subst prev0.
+        apply BLOCK.
+      }
+    }
+  Qed.
+
+  Theorem bb_elem_pred:
+    forall (header: node) (elem: node),
+      BasicBlock header elem ->
+        BasicBlockHeader elem
+        \/
+        forall (prev: node),
+          SuccOf f prev elem ->
+            BasicBlock header prev /\ Dominates f prev elem.
+  Proof.
+    intros header elem Hblock.
+    inversion Hblock.
+    { left. auto. }
+    {
+      right.
+      intros prev' Hsucc.
+      apply UNIQ in Hsucc.
+      subst prev'.
+      split; auto.
+      apply dom_path.
+      {
+        intros p Hpath.
+        inversion Hpath; subst. contradiction.
+        right.
+        apply UNIQ in HD. subst next.
+        apply (last_in_path f) with (x := entry). apply TL.
+      }
+      {
+        apply reach_succ with (a := prev). apply PRED.
+        apply bb_reaches with (header := header). apply BLOCK.
+      }
+    }
+  Qed.
+
+  Inductive BasicBlockSucc: node -> node -> Prop :=
+    | basic_block_succ:
+      forall (from: node) (to: node) (term: node)
+        (HDR_FROM: BasicBlock from term)
+        (HDR_TO: BasicBlockHeader to)
+        (SUCC: SuccOf f term to),
+        BasicBlockSucc from to
+    .
+
+  Inductive BasicBlockPath: node -> list node -> node -> Prop :=
+    | bb_path_nil:
+      forall (n: node)
+        (REACH: Reachable f n)
+        (HEADER: BasicBlockHeader n),
+        BasicBlockPath n [n] n
+    | bb_path_cons:
+      forall (from: node) (next: node) (to: node) (p: list node)
+        (REACH: Reachable f from)
+        (TL: BasicBlockPath from p next)
+        (HD: BasicBlockSucc next to),
+        BasicBlockPath from (to :: p) to
+    .
+
+  Inductive BasicBlockDominates: node -> node -> Prop :=
+    | bb_dom_self:
+      forall (n: node),
+        BasicBlockDominates n n
+    | bb_dom_path:
+      forall (a: node) (b: node)
+        (PATH: forall (p: list node), BasicBlockPath entry p b -> In a p)
+        (REACH: Reachable f b),
+        BasicBlockDominates a b
+    .
+
+  Theorem bb_dom_dom:
+    forall (n: node) (m: node),
+      BasicBlockDominates n m -> Dominates f n m.
+  Admitted.
+
+  Theorem bb_elem_dom:
+    forall (h: node) (e: node) (h': node) (e': node),
+      h <> h' ->
+      BasicBlock h e ->
+      BasicBlock h' e' ->
+      BasicBlockDominates h h' ->
+      Dominates f e e'.
+  Admitted.
+
+  Theorem bb_elem_not_header:
+    forall (h: node) (e: node),
+      BasicBlock h e ->
+      BasicBlockHeader e ->
+      h = e.
+  Proof.
+    intros h e Hbb Hheader.
+    inversion Hbb; auto.
+    subst header elem.
+    inversion Hheader.
+    apply TERM in PRED.
+    contradiction.
+  Qed.
+
+  Inductive SuccOfElem: node -> node -> Prop :=
+    | succ_of_elem:
+      forall (h: node) (n: node) (m: node)
+        (NH: m <> h)
+        (NE: n <> m)
+        (BN: BasicBlock h n)
+        (BM: BasicBlock h m)
+        (SUCC: SuccOf f n m),
+        SuccOfElem n m
+    .
+
+  Inductive PathToElem: node -> list node -> node -> Prop :=
+    | path_elem_header:
+      forall (n: node)
+        (HEADER: BasicBlockHeader n),
+        PathToElem n [n] n
+    | path_elem_cons:
+      forall (header: node) (prev: node) (elem: node) (p: list node)
+        (TL: SuccOfElem prev elem)
+        (HD: PathToElem header p prev)
+        (NH: header <> elem),
+        PathToElem header (elem :: p) elem
+    .
+
+  Theorem bb_path_to_elem:
+    forall (h: node) (e: node),
+      BasicBlock h e ->
+        exists (p: list node), PathToElem h p e.
+  Proof.
+    intros h e Hbb.
+    induction Hbb.
+    {
+      exists [header].
+      apply path_elem_header.
+      auto.
+    }
+    {
+      destruct IHHbb as [p Hpath].
+      exists (elem :: p).
+      apply path_elem_cons with (prev := prev); auto.
+      apply succ_of_elem with (h := header); auto.
+      apply bb_elem with (prev := prev); auto.
+    }
+  Qed.
+
+  Theorem bb_path_bb:
+    forall (h: node) (e: node) (p: list node),
+      PathToElem h p e -> BasicBlock h e.
+  Proof.
+    intros h e p Hpath.
+    induction Hpath.
+    + constructor; auto.
+    + inversion TL.
+      generalize (bb_header_unique prev header h IHHpath BN); intros Heq; subst.
+      apply bb_elem with (prev := prev);
+        inversion BM; subst; auto; try contradiction.
+      - apply UNIQ in SUCC; subst prev0; auto.
+      - intros prev' Hsucc.
+        apply UNIQ in Hsucc; subst prev'.
+        apply UNIQ in SUCC; subst prev.
+        reflexivity.
+  Qed.
+
+  Theorem bb_path_no_loop:
+    forall (h: node) (p: list node),
+      PathToElem h p h -> p = [h].
+  Proof.
+    intros h p Hpath.
+    inversion Hpath; auto.
+    subst. contradiction.
+  Qed.
+
+  Theorem bb_path_no_term:
+    forall (h: node) (e: node) (p: list node),
+      PathToElem h p e ->
+        forall (n: node),
+          In n p -> n = e \/ ~TermAt f n.
+  Proof.
+    intros h e p Hpath.
+    induction Hpath; intros n' Hin.
+    inversion Hin; auto.
+    destruct Hin; auto.
+    generalize (IHHpath n' H). intros Hind. clear IHHpath.
+    destruct Hind; auto.
+    inversion TL.
+    inversion BN; inversion BM; subst.
+    - contradiction.
+    - apply UNIQ in SUCC; subst; auto.
+    - contradiction.
+    - right. apply UNIQ0 in SUCC; subst; auto.
+  Qed.
+
+  Theorem bb_path_uniq:
+    forall (h: node) (e: node) (p: list node) (p': list node),
+      PathToElem h p e ->
+      PathToElem h p' e ->
+      p = p'.
+  Proof.
+    intros h e p p' Hp. generalize dependent p'.
+    induction Hp; intros p' Hp'.
+    symmetry; apply bb_path_no_loop; auto.
+    inversion Hp'; subst; try contradiction.
+    inversion TL; inversion TL0; inversion BM; subst; try contradiction.
+    apply UNIQ in SUCC; subst.
+    apply UNIQ in SUCC0; subst.
+    apply IHHp in HD; subst p0.
+    reflexivity.
+  Qed.
+
+  Definition get_bb_pred (e: node): option node :=
+    match get_predecessors f e with
+    | [p] =>
+      match f.(fn_insts) ! p with
+      | Some inst => if is_terminator inst then None else Some p
+      | None => None
+      end
+    | _ => None
+    end.
+
+  Theorem bb_header_has_no_predecessor:
+    forall (h: node),
+      BasicBlockHeader h ->
+      get_bb_pred h = None.
+  Proof.
+    intros h Hbb.
+    inversion Hbb.
+    unfold get_bb_pred.
+    remember (get_predecessors f h) as some_pred eqn:Esome_pred.
+    destruct some_pred; auto.
+    destruct some_pred; auto.
+    assert (Hk: SuccOf f k h).
+    {
+      apply get_predecessors_correct.
+      rewrite <- Esome_pred.
+      left; reflexivity.
+    }
+    inversion Hk.
+    rewrite <- HN.
+    apply TERM in Hk.
+    inversion Hk.
+    rewrite <- HN in INST0; inversion INST0; subst i0.
+    inversion TERM0; simpl; reflexivity.
+  Qed.
+
+  Theorem bb_elem_has_predecessor:
+    forall (h: node) (e: node),
+      BasicBlock h e ->
+      h <> e ->
+      exists (p: node), Some p = get_bb_pred e.
+  Proof.
+    intros h e Hbb Hne.
+    inversion Hbb; try contradiction.
+    exists prev.
+    unfold get_bb_pred.
+    remember (get_predecessors f e) as some_pred eqn:Esome_pred.
+    destruct some_pred.
+    {
+      apply get_predecessors_correct in PRED.
+      rewrite <- Esome_pred in PRED.
+      inversion PRED.
+    }
+    {
+      assert (Hk: SuccOf f k e).
+      {
+        apply get_predecessors_correct.
+        rewrite <- Esome_pred.
+        left. reflexivity.
+      }
+      destruct some_pred.
+      {
+        inversion Hk. apply UNIQ in Hk. rewrite <- HN.
+        inversion SUCC; simpl; subst k; try reflexivity;
+        (assert (TermAt f prev);
+        [ apply term_at with (i := i); auto; subst i; constructor
+        | contradiction
+        ]).
+      }
+      {
+        assert (Hk0: SuccOf f k0 e).
+        {
+          apply get_predecessors_correct.
+          rewrite <- Esome_pred.
+          right. left.  reflexivity.
+        }
+        apply UNIQ in Hk; subst k.
+        apply UNIQ in Hk0; subst k0.
+        unfold get_predecessors in Esome_pred.
+        destruct ((fn_insts f) ! e) eqn:E; try contradiction.
+        assert (Hdup: NoDup (prev :: prev :: some_pred)).
+        { unfold PTrie.key in *. rewrite Esome_pred. apply PTrie.keys_nodup. }
+        apply NoDup_cons_iff in Hdup. destruct Hdup as [Hdup _].
+        assert (Hcontra: In prev (prev :: some_pred)).
+        { left. reflexivity. }
+        contradiction.
+      }
+    }
+  Qed.
+
+  Theorem bb_elem_not_self:
+    forall (h: node) (e: node) (p: node),
+      BasicBlock h e ->
+      Some p = get_bb_pred e ->
+      p <> e.
+  Proof.
+    intros h e p Hblock Hsome contra.
+    subst p.
+    unfold get_bb_pred in Hsome.
+    remember (get_predecessors f e) as preds.
+    destruct preds; [inversion Hsome|].
+    destruct preds; [|inversion Hsome].
+    destruct ((fn_insts f) ! k) as [inst_k|] eqn:Einst_k; [|inversion Hsome].
+    assert (Hsucc: SuccOf f k e).
+    { apply get_predecessors_correct. rewrite <- Heqpreds. left. reflexivity. }
+    inversion Hblock; subst.
+    {
+      inversion HEADER.
+      apply TERM in Hsucc.
+      inversion Hsucc.
+      rewrite Einst_k in INST0; inversion INST0; subst i.
+      inversion TERM0; subst; simpl in Hsome; inversion Hsome.
+    }
+    {
+      apply UNIQ in Hsucc; subst k.
+      unfold is_terminator in Hsome.
+      destruct inst_k; inversion Hsome; subst e; contradiction.
+    }
+  Qed.
+
+  Theorem get_bb_pred_succ:
+    forall (n: reg) (m: reg),
+      get_bb_pred n = Some m -> SuccOf f m n.
+  Proof.
+    intros n m Hpred. unfold get_bb_pred in Hpred.
+    remember (get_predecessors f n) as preds.
+    destruct preds; [inversion Hpred|].
+    destruct preds; [|inversion Hpred].
+    destruct ((fn_insts f) ! k) as [pred|] eqn:Epred; [|inversion Hpred].
+    destruct pred; inversion Hpred; clear Hpred; subst k;
+    apply get_predecessors_correct;
+    rewrite <- Heqpreds;
+    left; reflexivity.
+  Qed.
+
+  Hypothesis has_header:
+    forall (e: node),
+      (exists (h: node), BasicBlock h e) \/ (f.(fn_insts) ! e = None).
+
+  Theorem  get_bb_pred_succ_of_elem:
+    forall (n: node) (m: node),
+      get_bb_pred n = Some m -> SuccOfElem m n.
+  Proof.
+    intros n m Hget.
+    unfold get_bb_pred in Hget.
+    remember (get_predecessors f n) as preds eqn:H.
+    destruct preds; [inversion Hget|].
+    destruct preds; [|inversion Hget].
+    destruct ((fn_insts f) ! k) as [inst_k|] eqn:Einst_k; [|inversion Hget].
+    assert (Hkm: k = m).
+    { destruct inst_k; simpl in Hget; inversion Hget; reflexivity. }
+    subst k.
+    generalize (has_header n); intros Hheader.
+    assert (Hsucc: SuccOf f m n).
+    { apply get_predecessors_correct. rewrite <- H. left. reflexivity. }
+    destruct Hheader as [[h Hbb]|Hnone].
+    {
+      inversion Hbb; subst.
+      {
+        inversion HEADER. apply TERM in Hsucc.
+        inversion Hsucc.
+        rewrite Einst_k in INST0; inversion INST0; clear INST0; subst i.
+        inversion TERM0; subst inst_k; simpl in Hget; inversion Hget.
+      }
+      {
+        apply succ_of_elem with (h := h); auto.
+        {
+          apply (bb_elem_not_self h); auto.
+          unfold get_bb_pred.
+          rewrite <- H; rewrite Einst_k; rewrite Hget; reflexivity.
+        }
+        { apply UNIQ in Hsucc; subst m; auto. }
+      }
+    }
+    {
+      unfold get_predecessors in H. rewrite Hnone in H. inversion H.
+    }
+  Defined.
+
+  Theorem succ_of_elem_wf: well_founded SuccOfElem.
+  Proof.
+    intros n.
+    generalize (has_header n); intros Hgraph; destruct Hgraph as [Hbb|Hnone].
+    {
+      destruct Hbb as [h Hbb].
+      induction Hbb.
+      {
+        constructor. intros y Hsucc.
+        inversion Hsucc; clear Hsucc; inversion HEADER; subst.
+        inversion SUCC.
+        inversion HEADER; subst.
+        inversion BM; subst.
+        { inversion HEADER0; subst; contradiction. }
+        { apply TERM in PRED; contradiction. }
+      }
+      {
+        constructor. intros y Hsucc.
+        assert (Hprevy: y = prev).
+        { apply UNIQ; inversion Hsucc; auto. }
+        subst y.
+        apply IHHbb.
+      }
+    }
+    {
+      constructor.
+      intros pred Hr.
+      inversion Hr; subst.
+      inversion BM.
+      { inversion HEADER; contradiction. }
+      { contradiction. }
+    }
+  Defined.
+
+  Function get_header (n: node) { wf SuccOfElem n }: node :=
+    match get_bb_pred n with
+    | Some n' => get_header n'
+    | None => n
+    end.
+    { apply get_bb_pred_succ_of_elem. }
+    { apply succ_of_elem_wf. }
+  Qed.
+
+  Function get_inst_index (n: node) { wf SuccOfElem n}: nat :=
+    match get_bb_pred n with
+    | Some n' => S (get_inst_index n')
+    | None => 0
+    end.
+    { apply get_bb_pred_succ_of_elem. }
+    { apply succ_of_elem_wf. }
+  Qed.
+
+  Theorem header_index_0:
+    forall (h: node),
+      BasicBlockHeader h -> get_inst_index h = 0.
+  Proof.
+    intros h Hbb.
+    rewrite get_inst_index_equation.
+    apply bb_header_has_no_predecessor in Hbb.
+    rewrite Hbb.
+    reflexivity.
+  Qed.
+End FUNCTION.
