State.v
@@ -1,8 +1,0 @@
-(* This file is part of the LLIR Semantics project. *)
-(* Licensing information is available in the LICENSE file. *)
-(* (C) 2020 Nandor Licker. All rights reserved. *)
-
-Require Import Coq.ZArith.ZArith.
-
-Require Import LLIR.Values.
-Require Import LLIR.Maps.
